spark2014_semantics/spark2014_core_subset/well_typed.v
@@ -1,43 +1,468 @@
 Require Export semantics_flagged.
 Require Export checks_optimization.
 
+Import STACK.
 
+
+(** * Helper Functions *)
+
+(** ** the type of the expression *)
+
+Definition type_of_name_x (st: symboltable_x) (n: name_x): option type :=
+  match n with
+  | E_Identifier_X ast_num _ _ => fetch_exp_type_x ast_num st
+  | E_Indexed_Component_X ast_num _ _ _ => fetch_exp_type_x ast_num st
+  | E_Selected_Component_X ast_num _ _ _ => fetch_exp_type_x ast_num st
+  end.
+
+Definition type_of_exp_x (st: symboltable_x) (e: expression_x): option type :=
+  match e with
+  | E_Literal_X _ (Integer_Literal _) _ _ => Some Integer
+  | E_Literal_X _ (Boolean_Literal _) _ _ => Some Boolean
+  | E_Name_X ast_num n => fetch_exp_type_x ast_num st
+  | E_Binary_Operation_X ast_num _ _ _ _ _ => fetch_exp_type_x ast_num st
+  | E_Unary_Operation_X ast_num _ _ _ _ => fetch_exp_type_x ast_num st
+  end.
+
+Definition binop_type (op: binary_operator) (t1 t2: type): option type :=
+    match op with
+    | Equal | Not_Equal | Greater_Than | Greater_Than_Or_Equal
+    | Less_Than | Less_Than_Or_Equal =>
+        match t1, t2 with
+        | Boolean, _ => None
+        | _, Boolean => None
+        | Array_Type _, _ => None
+        | _, Array_Type _ => None
+        | Record_Type _, _ => None
+        | _, Record_Type _ => None
+        | _, _ => Some Boolean
+        end
+    | And | Or =>
+        match t1, t2 with
+        | Boolean, Boolean => Some Boolean
+        | _, _ => None
+        end
+    | Plus | Minus | Multiply | Divide =>
+        match t1, t2 with
+        | Boolean, _ => None
+        | _, Boolean => None
+        | Array_Type _, _ => None
+        | _, Array_Type _ => None
+        | Record_Type _, _ => None
+        | _, Record_Type _ => None
+        | _, _ => Some Integer
+        end
+    end.
+
+Definition unop_type (op: unary_operator) (t: type): option type :=
+    match op with
+    | Unary_Minus =>
+        match t with
+        | Integer | Subtype _ | Derived_Type _ | Integer_Type _ => Some Integer
+        | _ => None
+        end
+    | Unary_Plus =>
+        Some t
+    | Not => 
+        match t with
+        | Boolean => Some Boolean
+        | _ => None
+        end
+    end.
+
+Definition type_match (t: type) (t': type) :=
+  match t with
+  | Boolean =>
+      match t' with
+      | Boolean => true
+      | _ => false
+      end
+  | Integer | Subtype _ | Derived_Type _ | Integer_Type _ => (* type match for assignment not exactly correct *)
+      match t' with
+      | Integer | Subtype _ | Derived_Type _ | Integer_Type _ => true
+      | _ => false
+      end
+  | Array_Type t1 =>
+      match t' with
+      | Array_Type t2 => beq_nat t1 t2
+      | _ => false
+      end
+  | Record_Type t1 =>
+      match t' with
+      | Record_Type t2 => beq_nat t1 t2
+      | _ => false
+      end
+  end.
+
+Lemma type_match_ref: forall t t',
+  type_match t t' = type_match t' t.
+Proof.
+  destruct t, t'; smack;
+  remember (beq_nat t t0) as b1;
+  remember (beq_nat t0 t) as b2;
+  destruct b1, b2; auto;
+  match goal with
+  | [H: true = beq_nat ?x ?y |- _] => rewrite (beq_nat_eq _ _ H) in *
+  end;
+  match goal with
+  | [H: _ = beq_nat ?x ?x |- _] => rewrite <- beq_nat_refl in H; inversion H
+  end.
+Qed.
+
+(** * Well-Typed Expression *)
+
+Inductive well_typed_exp_x: symboltable_x -> expression_x -> Prop :=
+  | WT_Literal_Int_X: forall st ast_num v in_cks ex_cks,
+      fetch_exp_type_x ast_num st = Some Integer ->
+      well_typed_exp_x st (E_Literal_X ast_num (Integer_Literal v) in_cks ex_cks)
+  | WT_Literal_Bool_X: forall st ast_num v in_cks ex_cks,
+      fetch_exp_type_x ast_num st = Some Boolean ->
+      well_typed_exp_x st (E_Literal_X ast_num (Boolean_Literal v) in_cks ex_cks)
+  | WT_Name_X: forall st ast_num n,
+      fetch_exp_type_x ast_num st = fetch_exp_type_x (name_astnum_x n) st ->
+      well_typed_name_x st n ->
+      well_typed_exp_x st (E_Name_X ast_num n)
+  | WT_Binary_Exp_X: forall st ast_num op e1 e2 in_cks ex_cks t t1 t2,
+      well_typed_exp_x st e1 ->
+      well_typed_exp_x st e2 ->
+      fetch_exp_type_x ast_num st = Some t -> (* binary expression's type *)
+      type_of_exp_x st e1 = Some t1 -> type_of_exp_x st e2 = Some t2 -> 
+      binop_type op t1 t2 = Some t -> (* binary expression's type *)
+      well_typed_exp_x st (E_Binary_Operation_X ast_num op e1 e2 in_cks ex_cks)
+  | WT_Unary_Exp_X: forall st ast_num op e in_cks ex_cks t t',
+      well_typed_exp_x st e ->
+      fetch_exp_type_x ast_num st = Some t -> (* unary expression's type *)
+      type_of_exp_x st e = Some t' ->
+      unop_type op t' = Some t -> (* unary expression's type *)
+      well_typed_exp_x st (E_Unary_Operation_X ast_num op e in_cks ex_cks)
+
+with well_typed_name_x: symboltable_x -> name_x -> Prop :=
+  | WT_Identifier_X: forall st ast_num x ex_cks md t,
+      fetch_exp_type_x ast_num st = Some t ->
+      fetch_var_x x st = Some (md, t) ->
+      well_typed_name_x st (E_Identifier_X ast_num x ex_cks)
+  | WT_Indexed_Component_X: forall st ast_num x e ex_cks t t' a_ast_num tn tm,
+      well_typed_name_x st x ->
+      well_typed_exp_x st e ->
+      fetch_exp_type_x ast_num st = Some t -> (* indexed component's type *)
+      fetch_exp_type_x (name_astnum_x x) st = Some (Array_Type t') ->
+      fetch_type_x t' st = Some (Array_Type_Declaration_X a_ast_num tn tm t) -> (* array element's type *)
+      well_typed_name_x st (E_Indexed_Component_X ast_num x e ex_cks)
+  | WT_Selected_Component_X: forall st ast_num x f ex_cks t t' r_ast_num tn fields,
+      well_typed_name_x st x ->
+      fetch_exp_type_x ast_num st = Some t -> (* selected component's type *)
+      fetch_exp_type_x (name_astnum_x x) st = Some (Record_Type t') ->
+      fetch_type_x t' st = Some (Record_Type_Declaration_X r_ast_num tn fields) ->
+      record_field_type fields f = Some t -> (* selected record field's type *)
+      well_typed_name_x st (E_Selected_Component_X ast_num x f ex_cks).
+
+Inductive well_typed_exps_x: symboltable_x -> list expression_x -> Prop :=
+  | WT_Exps_Nil_X: forall st,
+      well_typed_exps_x st nil
+  | WT_Exps_X: forall st e le,
+      well_typed_exp_x  st e  ->
+      well_typed_exps_x st le ->
+      well_typed_exps_x st (e :: le).
+
+Inductive well_typed_params_x: symboltable_x -> list parameter_specification_x -> Prop :=
+  | WT_Params_Nil_X: forall st,
+      well_typed_params_x st nil
+  | WT_Params_X: forall st m x lx,
+      fetch_var_x x.(parameter_name_x) st = Some (m, x.(parameter_subtype_mark_x)) ->
+      well_typed_params_x st lx ->
+      well_typed_params_x st (x :: lx).
+
+Inductive well_typed_args_x: symboltable_x -> list expression_x -> list parameter_specification_x -> Prop :=
+  | WT_Args_Nil_X: forall st,
+      well_typed_args_x st nil nil
+  | WT_Args_X: forall st e le x lx t,
+      fetch_exp_type_x (expression_astnum_x e) st = Some t ->
+      (* argument's type should match its parameter's type *)
+      type_match t x.(parameter_subtype_mark_x) = true ->
+      well_typed_args_x st le lx ->
+      well_typed_args_x st (e :: le) (x :: lx).
+
+(** * Well-Typed Statement *)
+
+Inductive well_typed_statement_x: symboltable_x -> statement_x -> Prop :=
+  | WT_Null_X: forall st,
+      well_typed_statement_x st S_Null_X
+  | WT_Assignment_X: forall st ast_num x e t t',
+      well_typed_exp_x st e ->
+      well_typed_name_x st x ->
+      fetch_exp_type_x (expression_astnum_x e) st = Some t ->
+      fetch_exp_type_x (name_astnum_x x) st = Some t' ->
+      (* +++ right-hand-side exp's type should be compatible with the left-hand-side exp's type *)
+      type_match t t' = true ->
+      well_typed_statement_x st (S_Assignment_X ast_num x e)
+  | WT_If_X: forall st ast_num e c1 c2,
+      well_typed_exp_x st e -> 
+      (* have to constrain that e is boolean or not ? *)
+      (* fetch_exp_type_x (expression_astnum_x e) st = Some Boolean -> *)
+      well_typed_statement_x st c1 ->
+      well_typed_statement_x st c2 ->
+      well_typed_statement_x st (S_If_X ast_num e c1 c2)
+  | WT_While_X: forall st ast_num e c,
+      well_typed_exp_x st e -> 
+      well_typed_statement_x st c ->
+      well_typed_statement_x st (S_While_Loop_X ast_num e c)
+  | WT_Procedure_Call_X: forall st ast_num f_ast_num f args n fb,
+      well_typed_exps_x st args ->
+      fetch_proc_x f st = Some (n, fb) ->
+      (* +++ the type of args shold match the type of params *)
+      well_typed_args_x st args (procedure_parameter_profile_x fb) ->
+      well_typed_statement_x st (S_Procedure_Call_X ast_num f_ast_num f args)
+  | WT_Sequence_X: forall st ast_num c1 c2,
+      well_typed_statement_x st c1 ->
+      well_typed_statement_x st c2 ->
+      well_typed_statement_x st (S_Sequence_X ast_num c1 c2).
+
+(** * Well-Typed Declaration *)
+
+Inductive well_typed_type_decl_x: symboltable_x -> type_declaration_x -> Prop :=
+  | WT_Subtype_Decl_X: forall st ast_num tid t r,
+      well_typed_type_decl_x st (Subtype_Declaration_X ast_num tid t r)
+  | WT_Derived_Type_Decl_X: forall st ast_num tid t r,
+      well_typed_type_decl_x st (Derived_Type_Declaration_X ast_num tid t r)
+  | WT_Int_Type_Decl_X: forall st ast_num tid r,
+      well_typed_type_decl_x st (Integer_Type_Declaration_X ast_num tid r)
+  | WT_Array_Type_Decl_X: forall st ast_num tid tm t,
+      well_typed_type_decl_x st (Array_Type_Declaration_X ast_num tid tm t)
+  | WT_Record_Type_Decl_X: forall st ast_num tid fs,
+      well_typed_type_decl_x st (Record_Type_Declaration_X ast_num tid fs).
+
+Inductive well_typed_decl_x: symboltable_x -> declaration_x -> Prop :=
+  | WT_Null_Decl_X: forall st,
+      well_typed_decl_x st D_Null_Declaration_X
+  | WT_Type_Decl_X: forall st ast_num type_decl,
+      well_typed_type_decl_x st type_decl ->
+      well_typed_decl_x st (D_Type_Declaration_X ast_num type_decl)
+  | WT_Object_Decl_None_Init_X: forall st ast_num d m,
+      d.(initialization_expression_x) = None ->
+      fetch_var_x d.(object_name_x) st = Some (m, d.(object_nominal_subtype_x)) ->
+      well_typed_decl_x st (D_Object_Declaration_X ast_num d)
+  | WT_Object_Decl_X: forall st ast_num d e m t,
+      d.(initialization_expression_x) = Some e ->
+      fetch_var_x d.(object_name_x) st = Some (m, d.(object_nominal_subtype_x)) ->
+      well_typed_exp_x st e ->
+      fetch_exp_type_x (expression_astnum_x e) st = Some t ->
+      (* type of the initialization expression should match the type of declared object *)
+      type_match t d.(object_nominal_subtype_x) = true ->
+      well_typed_decl_x st (D_Object_Declaration_X ast_num d)
+  | WT_Procedure_Body_X: forall st ast_num fb,
+      well_typed_proc_body_x st fb ->
+      well_typed_decl_x st (D_Procedure_Body_X ast_num fb)
+  | WT_Seq_Decl_X: forall st ast_num d1 d2,
+      well_typed_decl_x st d1 ->
+      well_typed_decl_x st d2 ->
+      well_typed_decl_x st (D_Seq_Declaration_X ast_num d1 d2)
+
+with well_typed_proc_body_x: symboltable_x -> procedure_body_x -> Prop :=
+  | WT_Proc_Body_X: forall st p,
+      well_typed_params_x st (procedure_parameter_profile_x p) ->
+      well_typed_decl_x st (procedure_declarative_part_x p) ->
+      well_typed_statement_x st (procedure_statements_x p) ->
+      well_typed_proc_body_x st p.
+
+(******************************************************************)
+(******************************************************************)
+
+(** * well typed symbol table *)
+
+(**
+  - Subtype_Declaration_X astnum typenum type range_x: "range_x" should be in the range of "type"
+  - Derived_Type_Declaration_X astnum typenum type range_x: "range_x" should be in the range of "type"
+  - Integer_Type_Declaration_X astnum typenum range_x: "range_x" should be in the range of "int32"
+  here in order to make the proof feasible, it's enough to have the subtype range within "int32"
+*)
+
+Inductive well_typed_subtype_declaration: symboltable_x -> Prop :=
+  | TSubtypeDecl: forall st, 
+ (* (forall t td l u, 
+      fetch_type_x t st = Some td ->
+        subtype_range_x td = Some (Range_X l u) ->
+          sub_bound (Interval l u) int32_bound true) -> *)
+    (forall t l u, 
+       extract_subtype_range_x st t (Range_X l u) ->
+         sub_bound (Interval l u) int32_bound true) ->
+    well_typed_subtype_declaration st.
+  
+Inductive well_typed_proc_declaration: symboltable_x -> Prop :=
+  | TProcDecl: forall st,
+    (forall f n p, fetch_proc_x f st = Some (n, p) -> 
+                   well_typed_proc_body_x st p) ->
+    well_typed_proc_declaration st.
+
+Inductive well_typed_symbol_table: symboltable_x -> Prop :=
+  | TSymbolTable: forall st, 
+      well_typed_subtype_declaration st ->
+      well_typed_proc_declaration st ->
+      well_typed_symbol_table st.
+
+
+(******************************************************************)
+(******************************************************************)
+
+(** * Well-Typed Value *)
+
+Inductive well_typed_value: symboltable_x -> type -> value -> Prop := 
+  | TV_Undefined: forall st t,
+      well_typed_value st t Undefined (*Undefined can be value of any type*)
+  | TV_Bool: forall st v,
+      v = true \/ v = false ->
+      well_typed_value st Boolean (Bool v)
+  | TV_Int: forall st v,
+      in_bound v int32_bound true ->
+      well_typed_value st Integer (Int v)
+  | TV_Subtype: forall st t l u v,
+      extract_subtype_range_x st (Subtype t) (Range_X l u) ->
+      in_bound v (Interval l u) true ->
+      well_typed_value st (Subtype t) (Int v)
+  | TV_Derived_Type: forall st t l u v,
+      extract_subtype_range_x st (Derived_Type t) (Range_X l u) ->
+      in_bound v (Interval l u) true ->
+      well_typed_value st (Derived_Type t) (Int v)
+  | TV_Integer_Type: forall st t l u v,
+      extract_subtype_range_x st (Integer_Type t) (Range_X l u) ->
+      in_bound v (Interval l u) true ->
+      well_typed_value st (Integer_Type t) (Int v)
+  | TV_Array_Type: forall st t ast_num tid tm typ a l u,
+      fetch_type_x t st = Some (Array_Type_Declaration_X ast_num tid tm typ) ->
+      extract_array_index_range_x st t (Range_X l u) ->
+      (forall i v, (* for value within the index range *)
+         array_select a i = Some v ->
+         (do_range_check i l u (Normal (Int i)) /\ well_typed_value st typ v)) ->
+      well_typed_value st (Array_Type t) (ArrayV a)
+  | TV_Record_Type: forall st t ast_num tid fields r,
+      fetch_type_x t st = Some (Record_Type_Declaration_X ast_num tid fields) ->
+      (* ????? *)
+      (*
+      (forall f v typ, 
+         record_select r f = Some v -> 
+         record_field_type fields f = Some typ -> (* selected record field's type *)
+         well_typed_value st typ v) ->
+      *)
+      (* ???? represented as the above or in the following way ??? *)
+      (forall f v, 
+         record_select r f = Some v -> 
+         exists typ, (record_field_type fields f = Some typ /\ well_typed_value st typ v)) ->
+      well_typed_value st (Record_Type t) (RecordV r).
+
+(** * Well-Typed Store *)
+Inductive well_typed_store: symboltable_x -> store -> Prop :=
+  | TStore: forall st s,
+      (forall x v,
+        fetches x s = Some v ->
+       exists m t, fetch_var_x x st = Some (m, t) /\ well_typed_value st t v) ->
+      well_typed_store st s.
+
+Inductive well_typed_value_in_store: symboltable_x -> store -> Prop :=
+  | TVStore_Nil: forall st,
+      well_typed_value_in_store st nil
+  | TVStore: forall st s x v,
+      (exists m t, fetch_var_x x st = Some (m, t) /\ well_typed_value st t v) ->
+      well_typed_value_in_store st s ->
+      well_typed_value_in_store st ((x, v) :: s).
+
+Lemma well_typed_store_infer: forall st s,
+  well_typed_value_in_store st s ->
+    well_typed_store st s.
+Proof.
+  intros st s; revert st.
+  induction s; intros.
+- constructor; smack.
+- inversion H; subst.
+  specialize (IHs _ H4).
+  constructor; smack.
+  remember (beq_nat x0 x) as b.
+  destruct b; smack.
+  + rewrite (beq_nat_eq _ _ Heqb).
+    exists x1 x2; smack.
+  + inversion IHs; smack.
+Qed.
+
+Ltac apply_well_typed_store_infer := 
+  match goal with
+  | [H: well_typed_value_in_store ?st ?s |- _] =>
+      specialize (well_typed_store_infer _ _ H);
+      let HZ := fresh "HZ" in intros HZ
+  end.
 
 (** * Well-Typed Stack *)
-Section Well_Typed_Stack_Sec.
-(** the value of variable and and record field are well-typed according to
-    the symbol table;
-
-  extract_array_index_range_x st arraytyp (Range_X l u) ->
-  do_range_check i l u Success ->
-  STACK.fetchG x s = Some (AggregateV (ArrayV a)) ->
-  array_select a i = Some (Int v) ->
-  valueO_of_array_component_type st arraytyp (IntBetween l' u') ->
-  (Zge_bool v l') && (Zle_bool v u') = true.
-
-
-
-  fetch_exp_type_x recAstNum st = Some (Record_Type t) ->
-  valueO_of_record_field_type st recType fieldId (IntBetween l u) ->
-  STACK.fetchG x s = Some (AggregateV (RecordV r)) ->
-  record_select r fieldId = Some (Int v) ->
-   (v >=? l)%Z && (v <=? u)%Z = true
-
-    TODO: to be completed !
+(** for any variable in stack, its value should be in the domain of its type;
+    for any procedure declaration in symbol table, the procedure is well-typed;
  *)
-Inductive well_typed_stack: symboltable_x -> STACK.stack -> Prop :=
-  | WTS: forall st s,
-      well_typed_stack st s. 
 
-(** for any variable in stack, its value should be in the domain of its type 
-    
-    TODO: to be proved !
+Inductive well_typed_stack: symboltable_x -> stack -> Prop :=
+  | TStack: forall st s,
+      (forall x v,
+         fetchG x s = Some v ->
+         exists m t, fetch_var_x x st = Some (m, t) /\ well_typed_value st t v) ->
+      well_typed_stack st s.
+
+Inductive well_typed_value_in_stack: symboltable_x -> stack -> Prop :=
+  | TVStack_Nil: forall st,
+      well_typed_value_in_stack st nil 
+  | TVStack: forall st s f, 
+      well_typed_value_in_store st (snd f) ->
+      well_typed_value_in_stack st s ->
+      well_typed_value_in_stack st (f :: s).
+
+Lemma well_typed_stack_infer: forall st s,
+  well_typed_value_in_stack st s ->
+    well_typed_stack st s.
+Proof.
+  intros st s; revert st.
+  induction s; intros.
+- constructor; smack.
+- inversion H; subst.
+  specialize (IHs _ H4).
+  constructor; smack.
+  remember (fetch x a) as y.
+  destruct y.
+  + inversion H0; subst.
+    apply_well_typed_store_infer.
+    inversion HZ; smack.
+  + inversion IHs; smack.
+Qed.
+
+Ltac apply_well_typed_stack_infer :=
+  match goal with
+  | [H: well_typed_value_in_stack ?st ?s |- _] =>
+      specialize (well_typed_stack_infer _ _ H);
+      let HZ := fresh "HZ" in intros HZ
+  end.
+
+(******************************************************************)
+(******************************************************************)
+
+(** * Well-Typed Stack and Symbol Table *)
+Inductive well_typed_stack_and_symboltable: symboltable_x -> stack -> Prop :=
+  | TStack_SymbolTable: forall st s,
+      well_typed_value_in_stack st s ->
+      well_typed_symbol_table st ->
+      well_typed_stack_and_symboltable st s.
+
+Ltac combine_well_typed_stack_and_symboltable := 
+  match goal with
+  | [H1: well_typed_value_in_stack ?st ?s,
+     H2: well_typed_symbol_table ?st |- _] =>
+      specialize (TStack_SymbolTable _ _ H1 H2); 
+      let HZ := fresh "HZ" in intros HZ
+  end.
+
+(*
+Inductive well_typed_stack: symboltable_x -> stack -> Prop :=
+  | TStack: forall st s,
+      (forall x v,
+         fetchG x s = Some v ->
+         exists m t, fetch_var_x x st = Some (m, t) /\ well_typed_value st t v) ->
+      (forall f n p, 
+         fetch_proc_x f st = Some (n, p) ->
+         well_typed_proc_body_x st p) ->
+      well_typed_stack st s.
 *)
-Axiom variable_value_in_type_domain: forall st s x_ast_num x ex_cks v t l u,
-  well_typed_stack st s ->
-    eval_name_x st s (E_Identifier_X x_ast_num x ex_cks) (Normal (Int v)) ->
-      fetch_exp_type_x x_ast_num st = Some t ->
-        bound_of_type st t (Interval l u) ->
-          (Zge_bool v l) && (Zle_bool v u) = true.
 
-End Well_Typed_Stack_Sec.
+
+
+
